fundamental property for the affine language

theories/examples/affine.v
@@ -2,10 +2,9 @@
 From Equations Require Import Equations.
 From iris.base_logic.lib Require Import na_invariants.
 From gitrees Require Import gitree program_logic.
-From gitrees.input_lang Require Import lang interp.
+From gitrees.input_lang Require Import lang interp logpred.
 From gitrees.examples Require Import store pairs.
 
-Definition s : stuckness := λ e, e = OtherError.
 
 Module io_lang.
   Definition state := input_lang.lang.state.
@@ -14,216 +13,16 @@ Module io_lang.
   Definition tyctx := tyctx ty.
   Definition typed {S} := input_lang.lang.typed (S:=S).
   Definition interp_closed {sz} (rs : gReifiers sz) `{!subReifier reify_io rs} (e : expr []) := input_lang.interp.interp_expr rs e ().
-
-Section io_lang.
-  Context {sz : nat}.
-  Variable rs : gReifiers sz.
-  Context `{!subReifier reify_io rs}.
-  Notation F := (gReifiers_ops rs).
-  Notation IT := (IT F).
-  Notation ITV := (ITV F).
-  Context `{!invGS Σ, !stateG rs Σ, !na_invG Σ}.
-  Notation iProp := (iProp Σ).
-
-  Variable p : na_inv_pool_name.
-
-  Program Definition interp_tnat : ITV -n> iProp := λne αv,
-    (∃ n, αv ≡ NatV n)%I.
-  Solve All Obligations with solve_proper.
-  Program Definition interp_tarr (Φ1 Φ2 : ITV -n> iProp) := λne αv,
-    (□ ∀ σ βv, has_substate σ -∗
-               na_own p ⊤ -∗
-               Φ1 βv -∗
-               WP@{rs} IT_of_V αv ⊙ (IT_of_V βv) @ s {{ v, ∃ σ', Φ2 v ∗ has_substate σ' ∗ na_own p ⊤ }})%I.
-  Solve All Obligations with solve_proper.
-
-  Fixpoint interp_ty (τ : ty) : ITV -n> iProp :=
-    match τ with
-    | Tnat => interp_tnat
-    | Tarr τ1 τ2 => interp_tarr (interp_ty τ1) (interp_ty τ2)
-    end.
-
-  Definition ssubst_valid {S} (Γ : tyctx S) (ss : ssubst S) : iProp :=
-    ([∗ list] τx ∈ zip (list_of_tyctx Γ) (list_of_ssubst (E:=F) ss),
-      interp_ty (τx.1) (τx.2))%I.
-
-  #[global] Instance io_lang_interp_ty_pers  τ βv : Persistent (io_lang.interp_ty τ βv).
-  Proof. induction τ; apply _. Qed.
-  #[global] Instance ssubst_valid_pers {S} (Γ : tyctx S) ss : Persistent (ssubst_valid  Γ  ss).
-  Proof. apply _. Qed.
-
-  Definition valid1 {S}  (Γ : tyctx S) (α : interp_scope S -n> IT) (τ : ty) : iProp :=
-    (∀ σ ss, has_substate σ -∗ na_own p ⊤ -∗ ssubst_valid Γ ss -∗
-          WP@{rs} α (interp_ssubst ss) @ s {{ v, ∃ σ', interp_ty τ v ∗ has_substate σ' ∗ na_own p ⊤ }}).
-
-  Lemma compat_nat {S} n (Ω : tyctx S) :
-    ⊢ valid1 Ω (interp_nat rs n) Tnat.
-  Proof.
-    iIntros (σ αs) "Hs Hp Has".
-    simpl. iApply wp_val. iModIntro. iFrame. eauto.
-  Qed.
-  Lemma compat_var {S} Ω τ (v : var S) :
-    typed_var Ω v τ →
-    ⊢ valid1 Ω (interp_var v) τ.
-  Proof.
-    intros Hv.
-    iIntros (σ ss) "Hs Hp Has".
-    unfold ssubst_valid.
-    iInduction Hv as [|? ? ? Ω v] "IH" forall (ss); simpl.
-    - dependent elimination ss as [cons_ssubst αv ss].
-      simp list_of_tyctx list_of_ssubst interp_ssubst.
-      simp interp_var. simpl.
-      iDestruct "Has" as "[H _]".
-      iApply wp_val; eauto with iFrame.
-    - dependent elimination ss as [cons_ssubst αv ss].
-      simp list_of_tyctx list_of_ssubst interp_ssubst.
-      simp interp_var. simpl.
-      iDestruct "Has" as "[_ H]".
-      by iApply ("IH" with "Hs Hp H").
-  Qed.
-  Lemma compat_if {S} (Γ : tyctx S) τ α β1 β2 :
-    ⊢ valid1 Γ α Tnat -∗
-      valid1 Γ β1 τ -∗
-      valid1 Γ β2 τ -∗
-      valid1 Γ (interp_if rs α β1 β2) τ.
-  Proof.
-    iIntros "H0 H1 H2".
-    iIntros (σ ss) "Hs Hp #Has".
-    iSpecialize ("H0" with "Hs Hp Has").
-    simpl. iApply (wp_bind _ (IFSCtx _ _)).
-    { solve_proper. }
-    iApply (wp_wand with "H0").
-    iIntros (αv) "Ha".
-    iDestruct "Ha" as (σ') "[Ha [Hs Hp]]".
-    iDestruct "Ha" as (n) "Hn".
-    iModIntro. unfold IFSCtx.
-    iRewrite "Hn".
-    destruct n as [|n].
-    - rewrite IF_False; last lia.
-      iApply ("H2" with "Hs Hp Has").
-    - rewrite IF_True; last lia.
-      iApply ("H1" with "Hs Hp Has").
-  Qed.
-  Lemma compat_input {S} (Γ : tyctx S) :
-    ⊢ valid1 Γ (interp_input rs) Tnat.
-  Proof.
-    iIntros (σ ss) "Hs Hp #Has".
-    simpl.
-    destruct (update_input σ) as [n σ'] eqn:Hinp.
-    iApply (wp_input with "Hs") .
-    { eauto. }
-    iNext. iIntros "_ Hs".
-    iApply wp_val. eauto with iFrame.
-  Qed.
-  Lemma compat_output {S} (Γ : tyctx S) α :
-    ⊢ valid1 Γ α Tnat → valid1 Γ (interp_output rs α) Tnat.
-  Proof.
-    iIntros "H". iIntros (σ ss) "Hs Hp #Has".
-    simpl.
-    iApply (wp_bind _ (get_nat _)).
-    { solve_proper. }
-    iSpecialize ("H" with "Hs Hp Has").
-    iApply (wp_wand with "H").
-    iIntros (αv) "Ha".
-    iDestruct "Ha" as (σ') "[Ha [Hs Hp]]".
-    iDestruct "Ha" as (n) "Hn".
-    iModIntro. iRewrite "Hn".
-    rewrite get_nat_nat.
-    iApply (wp_output with "Hs").
-    { reflexivity. }
-    iNext. iIntros "_ Hs".
-    eauto with iFrame.
-  Qed.
-  Lemma compat_app {S} (Γ : tyctx S) α β τ1 τ2 :
-    ⊢ valid1 Γ α (Tarr τ1 τ2) -∗
-      valid1 Γ β τ1 -∗
-      valid1 Γ (interp_app rs α β) τ2.
-  Proof.
-    iIntros "H1 H2".
-    iIntros (σ ss) "Hs Hp #Has". simpl.
-    iApply (wp_bind _  (AppRSCtx _)).
-    { solve_proper. }
-    iSpecialize ("H2" with "Hs Hp Has").
-    iApply (wp_wand with "H2").
-    iIntros (βv) "Hb".
-    iDestruct "Hb" as (σ') "[Hb [Hs Hp]]".
-    iModIntro. unfold AppRSCtx.
-    iApply (wp_bind _ (AppLSCtx (IT_of_V βv))).
-    { solve_proper. }
-    iSpecialize ("H1" with "Hs Hp Has").
-    iApply (wp_wand with "H1").
-    iIntros (αv) "Ha".
-    iDestruct "Ha" as (σ'') "[Ha [Hs Hp]]".
-    iModIntro. unfold AppLSCtx.
-    iApply ("Ha" with "Hs Hp Hb").
-  Qed.
-
-  Lemma compat_rec {S} (Γ : tyctx S) τ1 τ2 α :
-    ⊢ □ valid1 (consC (Tarr τ1 τ2) (consC τ1 Γ)) α τ2 -∗
-      valid1 Γ (interp_rec rs α) (Tarr τ1 τ2).
-  Proof.
-    iIntros "#H". iIntros (σ ss) "Hs Hp #Hss".
-    pose (env := (interp_ssubst ss)). fold env.
-    simp subst_expr.
-    pose (f := (ir_unf rs α env)).
-    iAssert (interp_rec rs α env ≡ IT_of_V $ FunV (Next f))%I as "Hf".
-    { iPureIntro. apply interp_rec_unfold. }
-    iRewrite "Hf".
-    iApply wp_val. iModIntro. iExists _. iFrame.
-    iLöb as "IH". iSimpl. iModIntro.
-    clear σ.
-    iIntros (σ βv) "Hs Hp #Hw".
-    iApply wp_lam.
-    iNext.
-    pose (ss' := cons_ssubst (FunV (Next f)) (cons_ssubst βv ss)).
-    iSpecialize ("H" $! _ ss' with "Hs Hp []").
-    { unfold ssubst_valid.
-      unfold ss'.
-      simp list_of_tyctx list_of_ssubst.
-      by iFrame "Hw IH Hss". }
-    unfold f. simpl.
-    unfold ss'. simp interp_ssubst.
-    iAssert (IT_of_V (FunV (Next f)) ≡ interp_rec rs α env)%I as "Heq".
-    { rewrite interp_rec_unfold. done. }
-    iRewrite -"Heq". iApply "H".
-  Qed.
-  Lemma fundamental {S} (Γ : tyctx S) e τ :
-    typed Γ e τ → ⊢ valid1 Γ (interp_expr rs e) τ
-  with fundamental_val {S} (Γ : tyctx S) v τ :
-    typed_val Γ v τ → ⊢ valid1 Γ (interp_val rs v) τ.
-  Proof.
-    - destruct 1.
-      + by iApply fundamental_val.
-      + by iApply compat_var.
-      + iApply compat_rec; iApply fundamental; eauto.
-      + iApply compat_app; iApply fundamental; eauto.
-      + admit.
-      + iApply compat_if;  iApply fundamental; eauto.
-      + iApply compat_input.
-      + iApply compat_output; iApply fundamental; eauto.
-    - destruct 1.
-      + iApply compat_nat.
-      + iApply compat_rec; iApply fundamental; eauto.
-  Admitted.
-  Lemma fundmanetal_closed (e : expr []) (τ : ty) :
-    typed empC e τ →
-    ⊢ valid1 empC (interp_expr rs e) τ.
-  Proof. apply fundamental. Qed.
-
 End io_lang.
-End io_lang.
-
-#[global] Instance io_lang_interp_ty_pers {sz} (rs : gReifiers sz)
-         `{!subReifier reify_io rs} `{!invGS Σ, !stateG rs Σ,!na_invG Σ} τ βv p
-  : Persistent (io_lang.interp_ty rs p τ βv).
-Proof. induction τ; apply _. Qed.
-
 
 
 Inductive ty :=
   tBool | tInt | tUnit
 | tArr (τ1 τ2 : ty) | tPair (τ1 τ2 : ty)
 | tRef (τ : ty).
+
+Local Notation tyctx := (tyctx ty).
+
 
 Inductive expr : scope → Type :=
 | LitBool (b : bool) {S} : expr S
@@ -232,13 +31,16 @@ Inductive expr : scope → Type :=
 | Lam {S} : expr (tt::S) → expr S
 | Var {S} : var S → expr S
 | App {S1 S2} : expr S1 → expr S2 → expr (S1++S2)
-(* | EPair {S} : expr S → expr S → expr S *)
-(* | EDestruct {S} : expr S → expr (()::()::S) → expr S *)
+| EPair {S1 S2} : expr S1 → expr S2 → expr (S1++S2)
+| EDestruct {S1 S2} : expr S1 → expr (()::()::S2) → expr (S1++S2)
+| Alloc {S} : expr S → expr S
+| Replace {S1 S2} : expr S1 → expr S2 → expr (S1++S2)
+| Dealloc {S} : expr S → expr S
 | EEmbed {S} : io_lang.expr [] → expr S
 .
 
-Local Notation tyctx := (tyctx ty).
 Inductive typed : forall {S}, tyctx  S → expr S → ty → Prop :=
+(** functions *)
 | typed_Var {S} (Ω : tyctx S) (τ : ty) (v : var S)  :
   typed_var Ω v τ →
   typed Ω (Var v) τ
@@ -249,6 +51,28 @@ Inductive typed : forall {S}, tyctx  S → expr S → ty → Prop :=
   typed Ω1 e1 (tArr τ1 τ2) →
   typed Ω2 e2 τ1 →
   typed (tyctx_app Ω1 Ω2) (App e1 e2) τ2
+(** pairs *)
+| typed_Pair {S1 S2} (Ω1 : tyctx S1) (Ω2 : tyctx S2) (τ1 τ2 : ty) e1 e2 :
+  typed Ω1 e1 τ1 →
+  typed Ω2 e2 τ2 →
+  typed (tyctx_app Ω1 Ω2) (EPair e1 e2) (tPair τ1 τ2)
+| typed_Destruct {S1 S2} (Ω1 : tyctx S1) (Ω2 : tyctx S2) (τ1 τ2 τ : ty)
+  (e1 : expr S1) (e2 : expr (()::()::S2)) :
+  typed Ω1 e1 (tPair τ1 τ2) →
+  typed (consC τ1 (consC τ2 Ω2)) e2 τ →
+  typed (tyctx_app Ω1 Ω2) (EDestruct e1 e2) τ
+(** references *)
+| typed_Alloc {S} (Ω : tyctx S) τ e :
+  typed Ω e τ →
+  typed Ω (Alloc e) (tRef τ)
+| typed_Replace {S1 S2} (Ω1 : tyctx S1) (Ω2 : tyctx S2) (τ1 τ2 : ty) e1 e2 :
+  typed Ω1 e1 (tRef τ1) →
+  typed Ω2 e2 τ2 →
+  typed (tyctx_app Ω1 Ω2) (Replace e1 e2) (tPair τ1 (tRef τ2))
+| typed_Dealloc {S} (Ω : tyctx S) e τ :
+  typed Ω e (tRef τ) →
+  typed Ω (Dealloc e) tUnit
+(** literals *)
 | typed_Nat {S} (Ω : tyctx S) n :
   typed Ω (LitNat n) tInt
 | typed_Bool {S} (Ω : tyctx S) b :
@@ -256,16 +80,6 @@ Inductive typed : forall {S}, tyctx  S → expr S → ty → Prop :=
 | typed_Unit {S} (Ω : tyctx S) :
   typed Ω LitUnit tUnit
 .
-
-Inductive ty_conv : ty → input_lang.lang.ty → Type :=
-| ty_conv_bool : ty_conv tBool Tnat
-| ty_conv_int  : ty_conv tInt  Tnat
-| ty_conv_unit : ty_conv tUnit Tnat
-| ty_conv_fun {τ1 τ2 t1 t2} :
-  ty_conv τ1 t1 → ty_conv τ2 t2 →
-  ty_conv (tArr τ1 τ2) (Tarr (Tarr Tnat t1) t2)
-.
-
 
 Section affine.
   Context {sz : nat}.
@@ -278,6 +92,12 @@ Section affine.
   Context `{!invGS Σ, !stateG rs Σ, !heapG rs Σ}.
   Notation iProp := (iProp Σ).
 
+  Variable s : stuckness.
+  Context `{A:ofe}.
+  Variable (P : A → iProp).
+  Context `{!NonExpansive P}.
+  Local Notation expr_pred := (expr_pred s rs P).
+
   Program Definition thunked : IT -n> locO -n> IT := λne e ℓ,
       λit _, IF (READ ℓ) (Err OtherError)
                          (SEQ (WRITE ℓ (Nat 1)) e).
@@ -285,11 +105,11 @@ Section affine.
   Program Definition thunkedV : IT -n> locO -n> ITV := λne e ℓ,
       FunV $ Next (λne _, IF (READ ℓ) (Err OtherError) (SEQ (WRITE ℓ (Nat 1)) e)).
   Solve All Obligations with first [solve_proper|solve_proper_please].
-  #[export] Instance tv_into_val e l : IntoVal (thunked e l) (thunkedV e l).
+  #[export] Instance thunked_into_val e l : IntoVal (thunked e l) (thunkedV e l).
   Proof.
-    unfold IntoVal. simpl. f_equiv. f_equiv. intro.
-    done.
+    unfold IntoVal. simpl. f_equiv. f_equiv. intro. done.
   Qed.
+
   Program Definition Thunk : IT -n> IT := λne e,
       ALLOC (Nat 0) (thunked e).
   Solve All Obligations with first [solve_proper|solve_proper_please].
@@ -303,20 +123,9 @@ Section affine.
     | Some l => Loc l
     | None   => Loc 0%Z
     end.
-  Program Definition interp_alloc {A} (α : A -n> IT) : A -n> IT := λne env,
-    LET (α env) $ λne α,
-    ALLOC α $ λne l, Nat (nat_of_loc l).
-  Solve All Obligations with solve_proper_please.
-  Program Definition interp_replace {A1 A2} (α : A1 -n> IT) (β : A2 -n> IT) : A1*A2 -n> IT := λne env,
-    LET (β env.2) $ λne β,
-    flip get_nat (α env.1) $ λ n,
-    LET (READ (loc_of_nat n)) $ λne γ,
-    SEQ (WRITE (loc_of_nat n) β) (pairT γ (Nat n)).
-  Solve All Obligations with solve_proper_please.
-  Program Definition interp_dealloc {A} (α : A -n> IT) : A -n> IT := λne env,
-    flip get_nat (α env) $ λ n,
-    DEALLOC (loc_of_nat n).
-  Solve All Obligations with solve_proper_please.
+
+  Lemma loc_of_nat_of_loc l : loc_of_nat (nat_of_loc l) = l.
+  Proof. Admitted.
 
   Definition interp_litbool (b : bool) {A} : A -n> IT := λne _,
     Nat (if b then 1 else 0).
@@ -325,7 +134,7 @@ Section affine.
   Definition interp_litunit {A} : A -n> IT := λne _, Nat 0.
   Program Definition interp_pair {A1 A2} (t1 : A1 -n> IT) (t2 : A2 -n> IT)
     : A1*A2 -n> IT := λne env,
-    pairT (t1 env.1) (t2 env.2).  (* we don't need to evaluate the pair here, i.e. lazy pairs? *)
+    pairIT (t1 env.1) (t2 env.2).  (* we don't need to evaluate the pair here, i.e. lazy pairs? *)
   Next Obligation. solve_proper_please. Qed.
   Program Definition interp_lam {A : ofe} (b : (IT * A) -n> IT) : A -n> IT := λne env,
     λit x, b (x,env).
@@ -337,23 +146,28 @@ Section affine.
     APP' f (Thunk x).
   Solve All Obligations with solve_proper_please.
   Program Definition interp_destruct {A1 A2 : ofe}
-       (ps : A1 -n> IT) (t : IT*IT*A2 -n> IT)
+       (ps : A1 -n> IT) (t : IT*(IT*A2) -n> IT)
     : A1*A2 -n> IT := λne env,
     LET (ps env.1) $ λne ps,
-    LET (Thunk (proj1T ps)) $ λne x,
-    LET (Thunk (proj2T ps)) $ λne y,
-    t (x, y, env.2).
+    LET (Thunk (projIT1 ps)) $ λne x,
+    LET (Thunk (projIT2 ps)) $ λne y,
+    t (x, (y, env.2)).
+  Solve All Obligations with solve_proper_please.
+  Program Definition interp_alloc {A} (α : A -n> IT) : A -n> IT := λne env,
+    LET (α env) $ λne α,
+    ALLOC α $ λne l, Nat (nat_of_loc l).
+  Solve All Obligations with solve_proper_please.
+  Program Definition interp_replace {A1 A2} (α : A1 -n> IT) (β : A2 -n> IT) : A1*A2 -n> IT := λne env,
+    LET (β env.2) $ λne β,
+    flip get_nat (α env.1) $ λ n,
+    LET (READ (loc_of_nat n)) $ λne γ,
+    SEQ (WRITE (loc_of_nat n) β) (pairIT γ (Nat n)).
+  Solve All Obligations with solve_proper_please.
+  Program Definition interp_dealloc {A} (α : A -n> IT) : A -n> IT := λne env,
+    flip get_nat (α env) $ λ n,
+    DEALLOC (loc_of_nat n).
   Solve All Obligations with solve_proper_please.
 
-  Definition interp_scope_split {S1 S2} {E} :
-    interp_scope (E:=E) (S1 ++ S2) -n> interp_scope (E:=E) S1 * interp_scope (E:=E) S2.
-  Proof.
-    induction S1 as [|? S1]; simpl.
-    - simple refine (λne x, (tt, x)).
-      solve_proper.
-    - simple refine (λne xy, let ss := IHS1 xy.2 in ((xy.1, ss.1), ss.2)).
-      solve_proper.
-  Defined.
 
   Fixpoint interp_expr {S} (e : expr S) : interp_scope S -n> IT :=
     match e with
@@ -363,18 +177,14 @@ Section affine.
     | Var v     => Force ◎ interp_var v
     | Lam e    => interp_lam (interp_expr e)
     | App e1 e2 => interp_app (interp_expr e1) (interp_expr e2) ◎ interp_scope_split
+    | EPair e1 e2 => interp_pair (interp_expr e1) (interp_expr e2) ◎ interp_scope_split
+    | EDestruct e1 e2 => interp_destruct (interp_expr e1) (interp_expr e2) ◎ interp_scope_split
+    | Alloc e => interp_alloc (interp_expr e)
+    | Dealloc e => interp_dealloc (interp_expr e)
+    | Replace e1 e2 => interp_replace (interp_expr e1) (interp_expr e2) ◎ interp_scope_split
     | EEmbed io_expr => constO (io_lang.interp_closed rs io_expr)
     end.
 
-
-  Context `{A:ofe}.
-  Variable (P : A → iProp).
-  Context `{!NonExpansive P}.
-
-  Program Definition expr_pred (α : IT) (Φ : ITV -n> iProp) : iProp :=
-    (∀ x : A, P x -∗ WP@{rs} α @ s {{ v, ∃ y : A, Φ v ∗ P y }}).
-  #[global] Instance expr_pred_ne : NonExpansive2 expr_pred.
-  Proof. solve_proper. Qed.
   (* interpreting tys *)
   Program Definition protected (Φ : ITV -n> iProp) : ITV -n> iProp := λne αv,
     (WP@{rs} Force (IT_of_V αv) @ s {{ Φ }})%I.
@@ -389,7 +199,7 @@ Section affine.
     (αv ≡ NatV 0)%I.
   Solve All Obligations with solve_proper_please.
   Program Definition interp_tpair (Φ1 Φ2 : ITV -n> iProp) : ITV -n> iProp := λne αv,
-    (∃ β1v β2v, IT_of_V αv ≡ pairTV (IT_of_V β1v) (IT_of_V β2v) ∗
+    (∃ β1v β2v, IT_of_V αv ≡ pairITV (IT_of_V β1v) (IT_of_V β2v) ∗
                        Φ1 β1v ∗ Φ2 β2v)%I.
   Solve All Obligations with solve_proper_please.
   Program Definition interp_tarr (Φ1 Φ2 : ITV -n> iProp) : ITV -n> iProp := λne αv,
@@ -410,103 +220,159 @@ Section affine.
     | tRef τ   => interp_ref (interp_ty τ)
     end.
 
-  Definition ssubst_valid {S} (Ω : tyctx S) (ss : ssubst S) : iProp :=
-    ([∗ list] τx ∈ zip (list_of_tyctx Ω) (list_of_ssubst (E:=F) ss),
-      protected (interp_ty (τx.1)) (τx.2))%I.
-
-
-  Equations ssubst_split {S1 S2} (αs : ssubst (E:=F) (S1++S2)) : ssubst (E:=F) S1 * ssubst (E:=F) S2 :=
-    ssubst_split (S1:=[]) αs := (emp_ssubst,αs);
-    ssubst_split (S1:=u::_) (cons_ssubst αv αs) := (cons_ssubst αv (ssubst_split αs).1, (ssubst_split αs).2).
-
-
-  Lemma ssubst_valid_app {S1 S2} (Ω1 : tyctx S1) (Ω2 : tyctx S2) αs :
-    ssubst_valid (tyctx_app Ω1 Ω2) αs ⊢ ssubst_valid Ω1 (ssubst_split αs).1
-                                      ∗ ssubst_valid Ω2 (ssubst_split αs).2.
-  Proof.
-    iInduction Ω1 as [|τ Ω1] "IH" forall (Ω2); simp tyctx_app ssubst_split.
-    - simpl. iIntros "$". unfold ssubst_valid.
-      simp list_of_ssubst list_of_tyctx. done.
-    - iIntros "H".
-      rewrite {4 5}/ssubst_valid.
-      simpl in αs.
-      dependent elimination αs as [cons_ssubst αv αs].
-      simp ssubst_split. simpl.
-      simp list_of_ssubst list_of_tyctx.
-      simpl. iDestruct "H" as "[$ H]".
-      by iApply "IH".
-  Qed.
-  Lemma interp_scope_ssubst_split {S1 S2} (αs : ssubst (S1++S2)) :
-    interp_scope_split (interp_ssubst αs) ≡
-      (interp_ssubst (ssubst_split αs).1, interp_ssubst (ssubst_split αs).2).
-  Proof.
-    induction S1 as [|u S1]; simpl.
-    - simp ssubst_split. simpl.
-      simp interp_ssubst. done.
-    - dependent elimination αs as [cons_ssubst αv αs].
-      simp ssubst_split. simpl.
-      simp interp_ssubst. repeat f_equiv; eauto; simpl.
-       + rewrite IHS1//.
-       + rewrite IHS1//.
-  Qed.
+  Definition ssubst_valid {S} (Ω : tyctx S) ss :=
+    lang_generic.ssubst_valid rs (λ τ, protected (interp_ty τ)) Ω ss.
 
   Definition valid1 {S} (Ω : tyctx S) (α : interp_scope S -n> IT) (τ : ty) : iProp :=
-    ∀ ss,  ssubst_valid Ω ss -∗ heap_ctx -∗ expr_pred (α (interp_ssubst ss)) (interp_ty τ).
+    ∀ ss, heap_ctx -∗ ssubst_valid Ω ss -∗ expr_pred (α (interp_ssubst ss)) (interp_ty τ).
+
+  Lemma compat_pair {S1 S2} (Ω1: tyctx S1) (Ω2:tyctx S2) α β τ1 τ2 :
+    ⊢ valid1 Ω1 α τ1 -∗
+      valid1 Ω2 β τ2 -∗
+      valid1 (tyctx_app Ω1 Ω2) (interp_pair α β ◎ interp_scope_split) (tPair τ1 τ2).
+  Proof.
+    Opaque pairITV.
+    iIntros "H1 H2".
+    iIntros (αs) "#Hctx Has".
+    cbn-[interp_pair].
+    unfold ssubst_valid.
+    rewrite ssubst_valid_app.
+    rewrite interp_scope_ssubst_split.
+    iDestruct "Has" as "[Ha1 Ha2]". cbn-[interp_app].
+    iSpecialize ("H1"  with "Hctx Ha1").
+    iSpecialize ("H2"  with "Hctx Ha2").
+    iApply (expr_pred_bind with "H2").
+    iIntros (βv) "Hb". simpl.
+    rewrite -> get_val_ITV. simpl.
+    iApply (expr_pred_bind with "H1").
+    iIntros (αv) "Ha". simpl.
+    rewrite -> get_val_ITV. simpl.
+    iApply expr_pred_ret.
+    iExists _,_. iFrame. done.
+  Qed.
+
+  Lemma wp_Thunk β  Φ `{!NonExpansive Φ}:
+    ⊢ heap_ctx -∗
+      ▷ (∀ l, pointsto l (Nat 0) -∗ Φ (thunkedV β l)) -∗
+      WP@{rs} Thunk β @ s {{ Φ }}.
+  Proof.
+    iIntros "#Hctx H".
+    iSimpl. iApply (wp_alloc with "Hctx").
+    iNext. iNext. iIntros (l) "Hl".
+    iApply wp_val. iModIntro.
+    iApply ("H" with "Hl").
+  Qed.
+  Opaque Thunk.
+
+  Lemma compat_destruct {S1 S2} (Ω1: tyctx S1) (Ω2:tyctx S2) α β τ1 τ2 τ :
+    ⊢ valid1 Ω1 α (tPair τ1 τ2) -∗
+      valid1 (consC τ1 $ consC τ2 Ω2) β τ -∗
+      valid1 (tyctx_app Ω1 Ω2) (interp_destruct α β ◎ interp_scope_split) τ.
+  Proof.
+    Opaque pairITV thunked thunkedV projIT1 projIT2.
+    iIntros "H1 H2".
+    iIntros (αs) "#Hctx Has".
+    cbn-[interp_destruct].
+    unfold ssubst_valid.
+    rewrite ssubst_valid_app.
+    rewrite interp_scope_ssubst_split.
+    iDestruct "Has" as "[Ha1 Ha2]".
+    iSpecialize ("H1"  with "Hctx Ha1").
+    simpl. iApply (expr_pred_bind (LETCTX _) with "H1").
+    iIntros (αv) "Ha". unfold LETCTX. simpl.
+    rewrite LET_Val/=.
+    iDestruct "Ha" as (β1 β2) "[#Ha [Hb1 Hb2]]".
+    iIntros (x) "Hx".
+    iApply wp_let.
+    { solve_proper. }
+    iApply (wp_Thunk with "Hctx").
+    { solve_proper_please. }
+    iNext. iIntros (l1) "Hl1". simpl.
+    iApply wp_let.
+    { solve_proper. }
+    iApply (wp_Thunk with "Hctx").
+    { solve_proper_please. }
+    iNext. iIntros (l2) "Hl2". simpl.
+    iSpecialize ("H2" $! (cons_ssubst (thunkedV (projIT1 (IT_of_V αv)) l1)
+                      $ cons_ssubst (thunkedV (projIT2 (IT_of_V αv)) l2) (ssubst_split αs).2)
+                with "Hctx [-Hx] Hx").
+    { unfold ssubst_valid. rewrite !ssubst_valid_cons.
+      iFrame. Transparent thunkedV thunked.
+      iSplitL "Hb1 Hl1".
+      - simpl. iApply wp_lam. simpl. iNext.
+        iApply (wp_bind _ (IFSCtx _ _)).
+        iApply (wp_read with "Hctx Hl1").
+        iNext. iNext. iIntros "Hl1".
+        iApply wp_val. iModIntro. unfold IFSCtx.
+        rewrite IF_False; last lia.
+        iApply wp_seq.
+        { solve_proper. }
+        iApply (wp_write with "Hctx Hl1").
+        iNext. iNext. iIntros "Hl1".
+        iRewrite "Ha".
+        rewrite projIT1_pairV. simpl.
+        repeat iApply wp_tick.
+        repeat iNext. iApply wp_val. done.
+      - simpl. iApply wp_lam. simpl. iNext.
+        iApply (wp_bind _ (IFSCtx _ _)).
+        iApply (wp_read with "Hctx Hl2").
+        iNext. iNext. iIntros "Hl2".
+        iApply wp_val. iModIntro. unfold IFSCtx.
+        rewrite IF_False; last lia.
+        iApply wp_seq.
+        { solve_proper. }
+        iApply (wp_write with "Hctx Hl2").
+        iNext. iNext. iIntros "Hl2".
+        iRewrite "Ha".
+        rewrite projIT2_pairV. simpl.
+        repeat iApply wp_tick.
+        repeat iNext. iApply wp_val. done.
+    }
+    simp interp_ssubst.
+    iApply "H2".
+  Qed.
 
   Lemma compat_alloc {S} (Ω : tyctx S) α τ:
     ⊢ valid1 Ω α τ -∗
       valid1 Ω (interp_alloc α) (tRef τ).
   Proof.
     iIntros "H".
-    iIntros (αs) "Has #Hctx".
-    iIntros (x) "Hx".
-    simpl.
-    iApply wp_let.
-    { solve_proper. }
-    iSpecialize ("H" with "Has Hctx Hx").
-    iApply (wp_wand with "H").
-    iIntros (αv). iDestruct 1 as (y) "[Ha Hx]".
-    iModIntro. simpl.
+    iIntros (αs) "#Hctx Has".
+    iSpecialize ("H" with "Hctx Has").
+    simpl. iApply (expr_pred_bind (LETCTX _) with "H").
+    iIntros (αv) "Hav". unfold LETCTX. simpl.
+    rewrite LET_Val/=.
+    iApply expr_pred_frame.
     iApply (wp_alloc with "Hctx").
-    { solve_proper. }
     iNext. iNext. iIntros (l) "Hl".
-    iApply wp_val.
-    iExists y. iFrame.
+    iApply wp_val. iModIntro. simpl.
     eauto with iFrame.
   Qed.
-
-  Lemma loc_of_nat_of_loc l : loc_of_nat (nat_of_loc l) = l.
-  Proof. Admitted.
 
   Lemma compat_replace {S1 S2} (Ω1 : tyctx S1) (Ω2 : tyctx S2) α β τ τ' :
     ⊢ valid1 Ω1 α (tRef τ) -∗
       valid1 Ω2 β τ' -∗
       valid1 (tyctx_app Ω1 Ω2) (interp_replace α β ◎ interp_scope_split) (tPair τ (tRef τ')).
   Proof.
-    Opaque pairTV.
+    Opaque pairITV.
     iIntros "H1 H2".
-    iIntros (αs) "Has #Hctx".
-    iIntros (x) "Hx". cbn-[interp_replace].
+    iIntros (αs) "#Hctx Has".
+    cbn-[interp_replace].
+    unfold ssubst_valid.
     rewrite ssubst_valid_app.
     rewrite interp_scope_ssubst_split.
     iDestruct "Has" as "[Ha1 Ha2]". cbn-[interp_app].
-    iSpecialize ("H1"  with "Ha1 Hctx").
-    iSpecialize ("H2"  with "Ha2 Hctx").
-    iApply wp_let.
-    { solve_proper. }
-    iSpecialize ("H2" with "Hx").
-    iApply (wp_wand with "H2").
-    iIntros (βv). iDestruct 1 as (y) "[Hb Hy]". iModIntro.
-    simpl.
-    iApply (wp_bind _ (get_nat _)).
-    { solve_proper. }
-    iSpecialize ("H1" with "Hy").
-    iApply (wp_wand with "H1").
-    iIntros (αv). iDestruct 1 as (z) "[Ha Hz]".
-    simpl.
+    iSpecialize ("H1"  with "Hctx Ha1").
+    iSpecialize ("H2"  with "Hctx Ha2").
+    iApply (expr_pred_bind (LETCTX _) with "H2").
+    iIntros (βv) "Hb". unfold LETCTX. simpl.
+    rewrite LET_Val/=.
+    iApply (expr_pred_bind with "H1").
+    iIntros (αv) "Ha". simpl.
     iDestruct "Ha" as (l γ) "[Ha [Hl Hg]]".
-    iModIntro. iRewrite "Ha".
-    rewrite get_nat_nat.
+    iApply expr_pred_frame.
+    iRewrite "Ha". simpl.
+    rewrite -> get_nat_nat.
     iApply wp_let.
     { solve_proper. }
     rewrite {1}loc_of_nat_of_loc.
@@ -521,7 +387,6 @@ Section affine.
     rewrite get_val_ITV. simpl.
     rewrite get_val_ITV. simpl.
     iApply wp_val. iModIntro.
-    iExists z; iFrame "Hz".
     iExists γ,(NatV (nat_of_loc l)).
     iSplit; first done.
     iFrame. eauto with iFrame.
@@ -532,17 +397,13 @@ Section affine.
       valid1 Ω (interp_dealloc α) tUnit.
   Proof.
     iIntros "H".
-    iIntros (αs) "Has #Hctx".
-    iIntros (x) "Hx".
-    simpl.
-    iApply (wp_bind _ (get_nat _)).
-    { solve_proper. }
-    iSpecialize ("H" with "Has Hctx Hx").
-    iApply (wp_wand with "H").
-    iIntros (αv). iDestruct 1 as (y) "[Ha Hx]".
-    iModIntro. simpl.
+    iIntros (αs) "#Hctx Has".
+    iSpecialize ("H" with "Hctx Has").
+    iApply (expr_pred_bind with "H").
+    iIntros (αv) "Ha /=".
     iDestruct "Ha" as (l βv) "[Ha [Hl Hb]]".
-    iRewrite "Ha". rewrite get_nat_nat.
+    iRewrite "Ha". iApply expr_pred_frame. simpl.
+    rewrite -> get_nat_nat.
     rewrite loc_of_nat_of_loc.
     iApply (wp_dealloc with "Hctx Hl").
     iNext. iNext. eauto with iFrame.
@@ -551,43 +412,40 @@ Section affine.
   Lemma compat_bool {S} b (Ω : tyctx S) :
     ⊢ valid1 Ω (interp_litbool b) tBool.
   Proof.
-    iIntros (αs) "Has #Hctx".
-    iIntros (x) "Hx".
-    simpl. iApply wp_val. iModIntro.
+    iIntros (αs) "#Hctx Has".
+    iApply expr_pred_ret.
     destruct b; simpl; eauto.
   Qed.
   Lemma compat_nat {S} n (Ω : tyctx S) :
     ⊢ valid1 Ω (interp_litnat n) tInt.
   Proof.
-    iIntros (αs) "Has #Hctx".
-    iIntros (x) "Hx".
-    simpl. iApply wp_val. iModIntro. eauto.
+    iIntros (αs) "#Hctx Has".
+    iApply expr_pred_ret. eauto with iFrame.
   Qed.
   Lemma compat_unit {S} (Ω : tyctx S) :
     ⊢ valid1 Ω interp_litunit tUnit.
   Proof.
-    iIntros (αs) "Has #Hctx".
-    iIntros (x) "Hx".
-    simpl. iApply wp_val. iModIntro. eauto.
+    iIntros (αs) "#Hctx Has".
+    iApply expr_pred_ret. eauto with iFrame.
   Qed.
-
   Lemma compat_var {S} Ω τ (v : var S) :
     typed_var Ω v τ →
     ⊢ valid1 Ω (Force ◎ interp_var v) τ.
   Proof.
-    iIntros (Hv ss) "Has #Hctx".
-    iIntros (x) "Hx".
+    iIntros (Hv ss) "#Hctx Has".
+    iApply expr_pred_frame.
     unfold ssubst_valid.
     iInduction Hv as [|? ? ? Ω v] "IH" forall (ss); simpl.
     - dependent elimination ss as [cons_ssubst αv ss].
-      simp list_of_tyctx list_of_ssubst interp_ssubst.
+      rewrite ssubst_valid_cons.
       simp interp_var. simpl.
       iDestruct "Has" as "[H _]".
-      iApply (wp_wand with "H"); eauto with iFrame.
+      simp interp_ssubst. simpl. done.
     - dependent elimination ss as [cons_ssubst αv ss].
-      simp list_of_tyctx list_of_ssubst interp_ssubst.
+      rewrite ssubst_valid_cons.
       simp interp_var. simpl.
       iDestruct "Has" as "[_ H]".
+      simp interp_ssubst. simpl.
       by iApply ("IH" with "H").
   Qed.
 
@@ -598,32 +456,23 @@ Section affine.
       valid1 (tyctx_app Ω1 Ω2) (interp_app α β ◎ interp_scope_split) τ2.
   Proof.
     iIntros "H1 H2".
-    iIntros (αs) "Has #Hctx".
-    iIntros (x) "Hx".
+    iIntros (αs) "#Hctx Has".
     iEval(cbn-[interp_app]).
+    unfold ssubst_valid.
     rewrite ssubst_valid_app.
     rewrite interp_scope_ssubst_split.
     iDestruct "Has" as "[Ha1 Ha2]". cbn-[interp_app].
-    iSpecialize ("H1"  with "Ha1 Hctx").
-    iSpecialize ("H2"  with "Ha2 Hctx").
+    iSpecialize ("H1"  with "Hctx Ha1").
+    iSpecialize ("H2"  with "Hctx Ha2").
     Local Opaque Thunk.
     iSimpl.
-    iApply wp_let.
-    { solve_proper. }
-    iSpecialize ("H2" with "Hx").
-    iApply (wp_wand with "H2").
-    iIntros (βv) "H2".
-    iDestruct "H2" as (y) "[H2 Hy]".
-    iModIntro. iSimpl.
-    iApply wp_let.
-    { solve_proper. }
-    iSpecialize ("H1" with "Hy").
-    iApply (wp_wand with "H1").
-    iIntros (αv) "H1".
-    iDestruct "H1" as (z) "[H1 Hz]".
-    iModIntro. simpl.
-    iSpecialize ("H1" with "H2 Hz").
-    iApply (wp_wand with "H1"). eauto with iFrame.
+    iApply (expr_pred_bind (LETCTX _) with "H2").
+    iIntros (βv) "H2". unfold LETCTX. iSimpl.
+    rewrite LET_Val/=.
+    iApply (expr_pred_bind (LETCTX _) with "H1").
+    iIntros (αv) "H1". unfold LETCTX. iSimpl.
+    rewrite LET_Val/=.
+    by iApply "H1".
   Qed.
 
   Lemma compat_lam {S} (Ω : tyctx S) τ1 τ2 α :
@@ -631,7 +480,7 @@ Section affine.
       valid1 Ω (interp_lam α) (tArr τ1 τ2).
   Proof.
     iIntros "H".
-    iIntros (αs) "Has #Hctx".
+    iIntros (αs) "#Hctx Has".
     iIntros (x) "Hx".
     iApply wp_val.
     iModIntro. simpl.
@@ -650,10 +499,9 @@ Section affine.
     iApply wp_lam. iNext.
     iEval(cbn-[thunked]).
     iSpecialize ("H" $! (cons_ssubst (thunkedV (IT_of_V βv) l) αs)
-             with "[-Hx] Hctx Hx").
+             with "Hctx [-Hx] Hx").
     { unfold ssubst_valid.
-      simp list_of_ssubst list_of_tyctx. simpl.
-      iFrame.
+      rewrite ssubst_valid_cons. iFrame.
       Local Transparent thunked thunkedV.
       iApply wp_lam. iNext. simpl.
       iApply (wp_bind _ (IFSCtx _ _)).
@@ -680,6 +528,11 @@ Section affine.
     - by iApply compat_var.
     - by iApply compat_lam.
     - by iApply compat_app.
+    - by iApply compat_pair.
+    - by iApply compat_destruct.
+    - by iApply compat_alloc.
+    - by iApply compat_replace.
+    - by iApply compat_dealloc.
     - by iApply compat_nat.
     - by iApply compat_bool.
     - by iApply compat_unit.
@@ -697,37 +550,77 @@ Section affine.
     iNext. iNext. iIntros (l) "Hl".
     iApply wp_val. iModIntro.
     unfold AppRSCtx.
-    rewrite tv_into_val.
+    rewrite thunked_into_val.
     iApply ("H" with "Hl").
   Qed.
 
-  Program Definition unsafe_fun : IT :=
-    ALLOC (Nat 42) $ λne l,
-      λit _, SEQ (DEALLOC l) (Nat 24).
-  Lemma unsafe_fun_valid :
-    ⊢ valid1 empC (constO unsafe_fun) (tArr tUnit tInt).
-  Proof.
-    iIntros (ss) "Hss #Hctx".
-    iIntros (x) "Hx".
-    unfold unsafe_fun. cbn-[interp_ty].
-    iApply (wp_alloc with "Hctx").
-    { solve_proper. }
-    iNext. iNext. iIntros (l) "H42".
-    iApply wp_val. iModIntro.
-    iExists x; iFrame. clear x.
-    iIntros (β) "Hb".
-    iIntros (x) "Hx".
-    iApply (wp_app_thunk with "Hctx").
-    { solve_proper. }
-    iNext. iIntros (t) "Ht".
-    iApply wp_lam. iNext. simpl.
-    iApply wp_seq.
-    { solve_proper. }
-    iApply (wp_dealloc with "Hctx H42").
-    iNext. iNext.
-    iApply wp_val. eauto with iFrame.
-  Qed.
 End affine.
+
+Arguments Force {_ _}.
+Arguments Thunk {_ _ _}.
+Arguments thunked {_ _ _}.
+Arguments thunkedV {_ _ _}.
+
+Arguments interp_tarr {_ _ _ _ _ _ _ _ _}.
+Arguments interp_ty {_ _ _ _ _ _ _ _ _ _} _.
+Local Arguments logpred.interp_tarr {_ _ _ _ _ _ _ _ _}.
+Local Arguments logpred.interp_ty {_ _ _ _ _ _ _ _ _} _.
+
+Inductive ty_conv : ty → io_lang.ty → Type :=
+| ty_conv_bool : ty_conv tBool Tnat
+| ty_conv_int  : ty_conv tInt  Tnat
+| ty_conv_unit : ty_conv tUnit Tnat
+| ty_conv_fun {τ1 τ2 t1 t2} :
+  ty_conv τ1 t1 → ty_conv τ2 t2 →
+  ty_conv (tArr τ1 τ2) (Tarr (Tarr Tnat t1) t2)
+.
+
+Inductive typed_glued : forall {S}, tyctx  S → expr S → ty → Type :=
+(** FFI *)
+| typed_Glue {S} (Ω : tyctx S) τ' τ e :
+  ty_conv τ τ' →
+  io_lang.typed empC e τ' →
+  typed_glued Ω (EEmbed e) τ
+(** functions *)
+| typed_VarG {S} (Ω : tyctx S) (τ : ty) (v : var S)  :
+  typed_var Ω v τ →
+  typed_glued Ω (Var v) τ
+| typed_LamG {S} (Ω : tyctx S) (τ1 τ2 : ty) (e : expr (()::S) ) :
+  typed_glued (consC τ1 Ω) e τ2 →
+  typed_glued Ω (Lam e) (tArr τ1 τ2)
+| typed_AppG {S1 S2} (Ω1 : tyctx S1) (Ω2 : tyctx S2) (τ1 τ2 : ty) e1 e2 :
+  typed_glued Ω1 e1 (tArr τ1 τ2) →
+  typed_glued Ω2 e2 τ1 →
+  typed_glued (tyctx_app Ω1 Ω2) (App e1 e2) τ2
+(** pairs *)
+| typed_PairG {S1 S2} (Ω1 : tyctx S1) (Ω2 : tyctx S2) (τ1 τ2 : ty) e1 e2 :
+  typed_glued Ω1 e1 τ1 →
+  typed_glued Ω2 e2 τ2 →
+  typed_glued (tyctx_app Ω1 Ω2) (EPair e1 e2) (tPair τ1 τ2)
+| typed_DestructG {S1 S2} (Ω1 : tyctx S1) (Ω2 : tyctx S2) (τ1 τ2 τ : ty)
+  (e1 : expr S1) (e2 : expr (()::()::S2)) :
+  typed_glued Ω1 e1 (tPair τ1 τ2) →
+  typed_glued (consC τ1 (consC τ2 Ω2)) e2 τ →
+  typed_glued (tyctx_app Ω1 Ω2) (EDestruct e1 e2) τ
+(** references *)
+| typed_AllocG {S} (Ω : tyctx S) τ e :
+  typed_glued Ω e τ →
+  typed_glued Ω (Alloc e) (tRef τ)
+| typed_ReplaceG {S1 S2} (Ω1 : tyctx S1) (Ω2 : tyctx S2) (τ1 τ2 : ty) e1 e2 :
+  typed_glued Ω1 e1 (tRef τ1) →
+  typed_glued Ω2 e2 τ2 →
+  typed_glued (tyctx_app Ω1 Ω2) (Replace e1 e2) (tPair τ1 (tRef τ2))
+| typed_DeallocG {S} (Ω : tyctx S) e τ :
+  typed_glued Ω e (tRef τ) →
+  typed_glued Ω (Dealloc e) tUnit
+(** literals *)
+| typed_NatG {S} (Ω : tyctx S) n :
+  typed_glued Ω (LitNat n) tInt
+| typed_BoolG {S} (Ω : tyctx S) b :
+  typed_glued Ω (LitBool b) tBool
+| typed_UnitG {S} (Ω : tyctx S) :
+  typed_glued Ω LitUnit tUnit
+.
 
 Section glue.
   Context {sz : nat}.
@@ -740,14 +633,13 @@ Section glue.
   Context `{!invGS Σ, !stateG rs Σ, !heapG rs Σ, !na_invG Σ}.
   Notation iProp := (iProp Σ).
 
-  Arguments Force {_ _}.
-  Arguments Thunk {_ _ _}.
-  Arguments thunked {_ _ _}.
-  Arguments thunkedV {_ _ _}.
-
+  Definition s : stuckness := λ e, e = OtherError.
   Variable p : na_inv_pool_name.
   Definition valid2 {S} (Ω : tyctx S) (α : interp_scope (E:=F) S -n> IT) (τ : ty) : iProp :=
-     valid1 rs (λ σ, has_substate σ ∗ na_own p ⊤)%I Ω α τ.
+     valid1 rs s (λ σ, has_substate σ ∗ na_own p ⊤)%I Ω α τ.
+
+  Definition io_valid {S} (Γ : io_lang.tyctx S) α (τ' : io_lang.ty) : iProp :=
+    input_lang.logpred.valid1 rs s (λ _ : unitO, na_own p ⊤) Γ α τ'.
 
   Program Definition glue_to_affine_fun (glue_from_affine glue_to_affine : IT -n> IT) : IT -n> IT := λne α,
     LET α $ λne α,
@@ -785,212 +677,301 @@ Section glue.
     | ty_conv_fun conv1 conv2 => glue_from_affine_fun (glue_from_affine conv2) (glue_to_affine conv1)
     end.
 
-(* Typeclasses Opaque thunkedV. *)
-Local Opaque thunked thunkedV Thunk.
-Lemma compat_glue_to_affine_bool {S} (Ω : tyctx S) α :
-  io_lang.valid1 rs p empC α Tnat ⊢
-  valid2 Ω (constO (glue2_bool (α ()))) tBool.
-Proof.
-  simpl.
-  iIntros "H". unfold io_lang.valid1.
-  iIntros (ss) "Has #Hctx". simpl.
-  iIntros (σ) "[Hs Hp]".
-  iSpecialize ("H" $! _ emp_ssubst with "Hs Hp []").
-  { unfold io_lang.ssubst_valid.
-    simp list_of_tyctx list_of_ssubst.
-    done. }
-  iApply (wp_bind _ (IFSCtx _ _)).
-  { solve_proper. }
-  iApply (wp_wand with "H").
-  iIntros (αv) "Ha". iDestruct "Ha" as (σ') "[Ha [Hs Hp]]".
-  iDestruct "Ha" as (n) "Ha".
-  iRewrite "Ha".
-  unfold IFSCtx.
-  iModIntro.
-  destruct n as [|n]; simpl.
-  * rewrite IF_False ; last lia.
-    iApply wp_val; eauto with iFrame.
-  * rewrite IF_True ; last lia.
-    iApply wp_val; eauto with iFrame.
-Qed.
-Lemma compat_glue_to_affine_nat {S} (Ω : tyctx S) α :
-  io_lang.valid1 rs p empC α Tnat ⊢
-  valid2 Ω (constO (α ())) tInt.
-Proof.
-  simpl.
-  iIntros "H". unfold io_lang.valid1.
-  iIntros (ss) "Has #Hctx". simpl.
-  iIntros (σ) "[Hs Hp]".
-  iSpecialize ("H" $! _ emp_ssubst with "Hs Hp []").
-  { unfold io_lang.ssubst_valid.
-    simp list_of_tyctx list_of_ssubst.
-    done. }
-  iApply (wp_wand with "H").
-  iIntros (αv) "Ha". iDestruct "Ha" as (σ') "[Ha Hs]".
-  eauto with iFrame.
-Qed.
-Lemma compat_glue_from_affine_bool α :
-  valid2 empC α tBool ⊢
-  heap_ctx -∗ io_lang.valid1 rs p empC α Tnat.
-Proof.
-  simpl.
-  iIntros "H #Hctx". unfold io_lang.valid1.
-  iIntros (σ ss) "Hs Hp Hss".
-  iSpecialize ("H" $! emp_ssubst with "[] Hctx [$Hs $Hp]").
-  { unfold ssubst_valid.
-    simp list_of_tyctx list_of_ssubst.
-    done. }
-  dependent elimination ss as [emp_ssubst].
-  iApply (wp_wand with "H").
-  iIntros (αv) "Ha". iDestruct "Ha" as (σ') "[Ha [Hs Hp]]".
-  iModIntro. iExists _; iFrame.
-  iDestruct "Ha" as "[Ha|Ha]"; iExists _; eauto.
-Qed.
-Lemma compat_glue_from_affine_nat α :
-  valid2 empC α tInt ⊢
-  heap_ctx -∗ io_lang.valid1 rs p empC α Tnat.
-Proof.
-  simpl.
-  iIntros "H #Hctx". unfold io_lang.valid1.
-  iIntros (σ ss) "Hs Hp Hss".
-  iSpecialize ("H" $! emp_ssubst with "[] Hctx [$Hs $Hp]").
-  { unfold ssubst_valid.
-    simp list_of_tyctx list_of_ssubst.
-    done. }
-  dependent elimination ss as [emp_ssubst].
-  iApply (wp_wand with "H").
-  iIntros (αv) "Ha". iDestruct "Ha" as (σ') "[Ha Hs]".
-  iModIntro. iExists _; iFrame.
-Qed.
-Lemma compat_glue_from_affine_unit α :
-  valid2 empC α tUnit ⊢
-  heap_ctx -∗ io_lang.valid1 rs p empC α Tnat.
-Proof.
-  simpl.
-  iIntros "H #Hctx". unfold io_lang.valid1.
-  iIntros (σ ss) "Hs Hp Hss".
-  iSpecialize ("H" $! emp_ssubst with "[] Hctx [$Hs $Hp]").
-  { unfold ssubst_valid.
-    simp list_of_tyctx list_of_ssubst.
-    done. }
-  dependent elimination ss as [emp_ssubst].
-  iApply (wp_wand with "H").
-  iIntros (αv) "Ha". iDestruct "Ha" as (σ') "[Ha [Hs Hp]]".
-  iModIntro. iExists _; iFrame.
-  iExists 0. iApply "Ha".
-Qed.
 
-Lemma compat_glue_to_affine_fun {S} (Ω : tyctx S) (τ1 τ2 : ty)
-  (τ1' τ2' : io_lang.ty) α (glue_to_affine glue_from_affine : IT -n> IT) :
-  (∀ α, io_lang.valid1 rs p empC α τ2'
-        ⊢ valid2 Ω (constO (glue_to_affine (α ()))) τ2) →
-  (∀ α,  valid2 empC (constO α) τ1
-        ⊢ heap_ctx -∗  io_lang.valid1 rs p empC
-                               (constO (glue_from_affine α)) τ1') →
-  io_lang.valid1 rs p empC α (Tarr (Tarr Tnat τ1') τ2')
-  ⊢ valid2 Ω
-      (constO (glue_to_affine_fun glue_from_affine glue_to_affine (α ())))
-      (tArr τ1 τ2).
-Proof.
-  intros G1 G2.
-  iIntros "H".
-  iIntros (αs) "Has #Hctx".
-  iIntros (σ) "[Hs Hp]".
-  simpl. iApply wp_let.
-  { solve_proper. }
-  iSpecialize ("H" $! _ emp_ssubst with "Hs Hp []").
-  { unfold io_lang.ssubst_valid.
-    simp list_of_tyctx list_of_ssubst.
-    done. }
-  iApply (wp_wand with "H").
-  iIntros (αv) "Ha". iDestruct "Ha" as (σ') "[Ha [Hs Hp]]".
-  iSimpl in "Ha". iDestruct "Ha" as "#Ha".
-  iSimpl. iModIntro.
-  iApply wp_val. iModIntro.
-  simpl. iExists σ'. iFrame.
-  iIntros (βv) "Hb".
-  (* preparing a thunk *)
-  iSimpl. clear σ.
-  iIntros (σ) "[Hs Hp]".
-  iApply (wp_bind _ (AppRSCtx _)).
-  { solve_proper. }
-  iApply (wp_alloc with "Hctx").
-  { solve_proper. }
-  iNext. iNext. iIntros (l) "Hl".
-  iApply wp_val. iModIntro.
-  unfold AppRSCtx.
-  iApply wp_lam. iNext.
-  iEval(cbn-[thunked]).
-  iApply wp_let.
-  { solve_proper. }
-  iApply wp_lam.
-  (* forcing a thunk *)
-  iNext. iSimpl.
-  iApply (wp_bind _ (IFSCtx _ _)).
-  { solve_proper. }
-  iApply (wp_read with "Hctx Hl").
-  iNext. iNext. iIntros "Hl".
-  iApply wp_val. iModIntro.
-  unfold IFSCtx. simpl.
-  rewrite IF_False; last lia.
-  iApply wp_seq.
-  { solve_proper. }
-  iApply (wp_write with "Hctx Hl").
-  iNext. iNext. iIntros "Hl".
-  iApply wp_val. iModIntro.
-  (* doing the glue for the argument *)
-  iApply (wp_let).
-  { solve_proper. }
-  iPoseProof (G2 (IT_of_V βv)) as "G2".
-  iSpecialize ("G2" with "[Hb]").
-  { iIntros (ss) "Hss _".
-    iIntros (σ0) "Hs". simpl.
-    iApply wp_val. eauto with iFrame. }
-  iSpecialize ("G2" with "Hctx").
-  iSpecialize ("G2" $! _ emp_ssubst with "Hs Hp []").
-  { unfold io_lang.ssubst_valid.
-    simp list_of_tyctx list_of_ssubst.
-    done. }
-  iApply (wp_wand with "G2").
-  iIntros (β'v) "Hb". iModIntro.
-  simpl. clear σ σ'. iDestruct "Hb" as (σ) "[#Hb [Hs Hp]]".
-  (* calling the original function *)
-  iApply wp_let.
-  { solve_proper. }
-  iApply (wp_bind _ (AppRSCtx _)).
-  { solve_proper. }
-  iApply (wp_alloc with "Hctx").
-  { solve_proper. }
-  iNext. iNext. iIntros (l') "Hl'".
-  iApply (wp_val _ _ (thunkedV _ _)).
-  iModIntro.
-  unfold AppRSCtx.
-  iClear "Hl". clear l.
-  iApply fupd_wp.
-  { solve_proper. }
-  iMod (inv_alloc (nroot.@"yolo") _ (∃ n, pointsto l' (Nat n)) with "[Hl']") as "#Hinv".
-  { iNext. iExists _; done. }
-  iPoseProof ("Ha" $! _ (thunkedV (IT_of_V β'v) l') with "Hs Hp [-Has]") as "H1".
-  { iModIntro. iIntros (σ' βn) "Hs Hp".
-    iDestruct 1 as (m) "Hbm".
-    iApply wp_lam. iNext. iSimpl.
+  Local Opaque thunked thunkedV Thunk.
+  Lemma compat_glue_to_affine_bool {S} (Ω : tyctx S) α :
+    io_valid empC α Tnat ⊢
+     valid2 Ω (constO (glue2_bool (α ()))) tBool.
+  Proof.
+    iIntros "H".
+    iIntros (ss) "#Hctx Has". simpl.
+    iIntros (σ) "[Hs Hp]".
+    iSpecialize ("H" $! σ emp_ssubst with "Hs []").
+    { unfold logpred.ssubst_valid.
+      iApply ssubst_valid_nil. }
+    iSpecialize ("H" $! tt with "Hp").
+    simp interp_ssubst. simpl.
     iApply (wp_bind _ (IFSCtx _ _)).
     { solve_proper. }
-    iApply (wp_read_atomic _ _ (⊤∖ nclose (nroot.@"storeE")) with "Hctx").
-    { set_solver. }
-    iInv (nroot.@"yolo") as (n) "Hl'" "Hcl".
-    iModIntro. iExists (Nat n). iFrame.
-    iNext. iNext. iIntros "Hl'".
-    iMod ("Hcl" with "[Hl']") as "_".
-    { iNext. eauto with iFrame. }
-    iModIntro. iApply wp_val.
+    iApply (wp_wand with "H").
+    iIntros (αv). iDestruct 1 as (_) "[Ha Hp]".
+    iDestruct "Ha" as (σ') "[Ha Hs]".
+    iDestruct "Ha" as (n) "Ha".
+    iRewrite "Ha".
+    unfold IFSCtx.
+    iModIntro. destruct n as [|n]; simpl.
+    * rewrite IF_False ; last lia.
+      iApply wp_val; eauto with iFrame.
+    * rewrite IF_True ; last lia.
+      iApply wp_val; eauto with iFrame.
+  Qed.
+  Lemma compat_glue_to_affine_nat {S} (Ω : tyctx S) α :
+    io_valid empC α Tnat ⊢
+      valid2 Ω (constO (α ())) tInt.
+  Proof.
+    iIntros "H".
+    iIntros (ss) "#Hctx Has". simpl.
+    iIntros (σ) "[Hs Hp]".
+    iSpecialize ("H" $! σ emp_ssubst with "Hs []").
+    { unfold logpred.ssubst_valid.
+      iApply ssubst_valid_nil. }
+    iSpecialize ("H" $! tt with "Hp").
+    simp interp_ssubst. simpl.
+    iApply (wp_wand with "H").
+    iIntros (αv). iDestruct 1 as (_) "[Ha Hp]".
+    iDestruct "Ha" as (σ') "[Ha Hs]".
+    iModIntro. eauto with iFrame.
+
+  Qed.
+  Lemma compat_glue_from_affine_bool α :
+    valid2 empC α tBool ⊢
+      heap_ctx -∗ io_valid empC α Tnat.
+  Proof.
+    iIntros "H #Hctx".
+    iIntros (σ ss) "Hs Hss".
+    iIntros (_) "Hp".
+    iSpecialize ("H" $! emp_ssubst with "Hctx [] [$Hs $Hp]").
+    { iApply ssubst_valid_nil. }
+    dependent elimination ss as [emp_ssubst].
+    iApply (wp_wand with "H").
+    iIntros (αv) "Ha". iDestruct "Ha" as (σ') "[Ha [Hs Hp]]".
+    iModIntro. simpl. iFrame. iExists tt,_; iFrame.
+    iDestruct "Ha" as "[Ha|Ha]"; iExists _; eauto.
+  Qed.
+  Lemma compat_glue_from_affine_nat α :
+    valid2 empC α tInt ⊢
+      heap_ctx -∗ io_valid empC α Tnat.
+  Proof.
+    iIntros "H #Hctx".
+    iIntros (σ ss) "Hs Hss".
+    iIntros (_) "Hp".
+    iSpecialize ("H" $! emp_ssubst with "Hctx [] [$Hs $Hp]").
+    { iApply ssubst_valid_nil. }
+    dependent elimination ss as [emp_ssubst].
+    iApply (wp_wand with "H").
+    iIntros (αv) "Ha". iDestruct "Ha" as (σ') "[Ha [Hs Hp]]".
+    iModIntro. iExists tt. eauto with iFrame.
+  Qed.
+  Lemma compat_glue_from_affine_unit α :
+    valid2 empC α tUnit ⊢
+      heap_ctx -∗ io_valid empC α Tnat.
+  Proof.
+    iIntros "H #Hctx".
+    iIntros (σ ss) "Hs Hss".
+    iIntros (_) "Hp".
+    iSpecialize ("H" $! emp_ssubst with "Hctx [] [$Hs $Hp]").
+    { iApply ssubst_valid_nil. }
+    dependent elimination ss as [emp_ssubst].
+    iApply (wp_wand with "H").
+    iIntros (αv) "Ha". iDestruct "Ha" as (σ') "[Ha [Hs Hp]]".
+    iModIntro. iExists tt. iFrame. simpl.
+    iRewrite "Ha". eauto with iFrame.
+  Qed.
+
+  Local Opaque interp_tarr logpred.interp_tarr.
+
+  Lemma compat_glue_from_affine_fun (τ1 τ2 : ty)
+    (τ1' τ2' : io_lang.ty) α (glue_to_affine glue_from_affine : IT -n> IT) :
+    (∀ α, io_valid empC α τ1'
+            ⊢ valid2 empC (constO (glue_to_affine (α ()))) τ1) →
+    (∀ α,  valid2 empC (constO α) τ2
+             ⊢ heap_ctx -∗ io_valid empC (constO (glue_from_affine α)) τ2') →
+    valid2 empC (constO α) (tArr τ1 τ2)
+    ⊢ heap_ctx -∗
+      io_valid empC
+         (constO (glue_from_affine_fun glue_from_affine glue_to_affine α))
+         (Tarr (Tarr Tnat τ1') τ2').
+  Proof.
+    intros G1 G2.
+    iIntros "H #Hctx". iIntros (σ ss) "Hs _ _ Hp".
+    simpl. clear ss.
+    iSpecialize ("H" $! emp_ssubst with "Hctx [] [$Hs $Hp]").
+    { iApply ssubst_valid_nil. }
+    simpl. iApply wp_let.
+    { solve_proper. }
+    iApply (wp_wand with "H").
+    iIntros (αv) "Ha". iDestruct "Ha" as (σ') "[Ha [Hs Hp]]".
+    iSimpl in "Ha".
+    iSimpl. iModIntro.
+    iApply wp_let.
+    { solve_proper. }
+    iApply (wp_Thunk with "Hctx").
+    { solve_proper_please. }
+    iNext. iIntros (l) "Hl".
+    iApply fupd_wp.
+    { solve_proper. }
+    iMod (na_inv_alloc p _ (nroot.@"yolo")
+            (pointsto l (Nat 1) ∨
+               (pointsto l (Nat 0) ∗ interp_tarr (interp_ty τ1) (interp_ty τ2) αv)) with "[Hl Ha]") as "#Hinv".
+    { iNext. iRight. iFrame. }
+    iModIntro. simpl. iApply wp_val.
+    iModIntro. iExists tt. iFrame. iExists σ'. iFrame.
+    iModIntro. clear σ σ'. iIntros (σ βv) "Hs #Hb".
+    iIntros (_) "Hp".
+    iApply wp_lam. iNext. simpl.
+    iApply wp_let.
+    { solve_proper. }
+    iApply wp_lam. iNext. simpl.
+    iApply (wp_bind _ (IFSCtx _ _)).
+    { solve_proper_please. }
+    iApply fupd_wp.
+    { solve_proper. }
+    iMod  (na_inv_acc with "Hinv Hp")
+      as "[Hl [Hp Hcl]]"; [ set_solver | set_solver | ].
     iModIntro.
-    unfold IFSCtx. simpl.
-    destruct n as [|n].
-    - rewrite IF_False; last lia.
+    iDestruct "Hl" as "[Hl | [Hl Ha]]".
+    * iApply (wp_read with "Hctx Hl").
+      iNext. iNext. iIntros "Hl".
+      iApply wp_val.
+      iModIntro.
+      unfold IFSCtx. simpl.
+      rewrite IF_True; last lia.
+      iApply wp_err. done.
+    * iApply (wp_read with "Hctx Hl").
+      iNext. iNext. iIntros "Hl".
+      iApply wp_val.
+      iModIntro.
+      unfold IFSCtx. simpl.
+      rewrite IF_False; last lia.
       iApply wp_seq.
+      { solve_proper_please. }
+      iApply (wp_write with "Hctx Hl").
+      iNext. iNext. iIntros "Hl".
+      iApply wp_val.
+      iMod ("Hcl" with "[Hl $Hp]") as "Hp".
+      { iNext. iLeft; eauto. }
+      iModIntro.
+      iApply wp_let.
       { solve_proper. }
-      iApply (wp_write_atomic _ _ (⊤∖ nclose (nroot.@"storeE")) with "Hctx").
+      iSpecialize ("Hb" $! _ (NatV 0) with "Hs []").
+      { eauto with iFrame. }
+      iSpecialize ("Hb" $! tt with "Hp").
+      iApply (wp_wand with "Hb").
+      iIntros (γv). iDestruct 1 as (_) "[Hg Hp]".
+      iDestruct "Hg" as (σ') "[Hg Hst]".
+      iModIntro. simpl.
+      iApply wp_let.
+      { solve_proper. }
+      iPoseProof (G1 (constO (IT_of_V γv))) as "G1".
+      iSpecialize ("G1" with "[Hg]").
+      { iIntros (σ0 ss0) "Hs Has". simpl.
+        iApply expr_pred_ret. simpl. eauto with iFrame. }
+      iSpecialize ("G1" $! emp_ssubst with "Hctx [] [$Hst $Hp]").
+      { iApply ssubst_valid_nil. }
+      iApply (wp_wand with "G1").
+      clear βv σ'.
+      iIntros (βv). iDestruct 1 as (σ') "[Hb [Hst Hp]]".
+      iModIntro. simpl.
+      iApply wp_let.
+      { solve_proper. }
+      iSpecialize ("Ha" with "Hb [$Hst $Hp]").
+      iApply (wp_wand with "Ha").
+      clear γv σ'.
+      iIntros (γv). iDestruct 1 as (σ') "[Hg [Hst Hp]]".
+      iModIntro.
+      iPoseProof (G2 (IT_of_V γv)) as "G1".
+      iSpecialize ("G1" with "[Hg] Hctx").
+      { iIntros (ss0) "_ _".
+        by iApply expr_pred_ret. }
+      iSpecialize ("G1" $! _ emp_ssubst with  "Hst []").
+      { iApply ssubst_valid_nil. }
+      iApply ("G1" $! tt with "Hp").
+  Qed.
+
+  Lemma compat_glue_to_affine_fun {S} (Ω : tyctx S) (τ1 τ2 : ty)
+    (τ1' τ2' : io_lang.ty) α (glue_to_affine glue_from_affine : IT -n> IT) :
+    (∀ α, io_valid empC α τ2'
+            ⊢ valid2 Ω (constO (glue_to_affine (α ()))) τ2) →
+    (∀ α,  valid2 empC (constO α) τ1
+             ⊢ heap_ctx -∗ io_valid empC (constO (glue_from_affine α)) τ1') →
+    io_valid empC α (Tarr (Tarr Tnat τ1') τ2')
+      ⊢ valid2 Ω
+      (constO (glue_to_affine_fun glue_from_affine glue_to_affine (α ())))
+      (tArr τ1 τ2).
+  Proof.
+    intros G1 G2.
+    iIntros "H".
+    iIntros (αs) "#Hctx Has".
+    iIntros (σ) "[Hs Hp]". simpl.
+    iSpecialize ("H" $! _ emp_ssubst with "Hs []").
+    { iApply ssubst_valid_nil. }
+    iSpecialize ("H" $! tt with "Hp").
+    simp interp_ssubst. simpl.
+    iApply wp_let.
+    { solve_proper. }
+    iApply (wp_wand with "H").
+    iIntros (αv). iDestruct 1 as (_) "[Ha Hp]".
+    iDestruct "Ha" as (σ') "[Ha Hs]".
+    simpl. iModIntro.
+    iApply wp_val. iModIntro.
+    iExists σ'. iFrame.
+    iIntros (βv) "Hb".
+    (* preparing a thunk *)
+    iSimpl. clear σ σ'.
+    iIntros (σ) "[Hs Hp]".
+    iApply (wp_bind _ (AppRSCtx _)).
+    { solve_proper. }
+    iApply (wp_Thunk with "Hctx").
+    { solve_proper. }
+    iNext. iIntros (l) "Hl".
+    unfold AppRSCtx.
+    iApply wp_lam. iNext.
+    iEval(cbn-[thunked]).
+    iApply wp_let.
+    { solve_proper. }
+    iApply wp_lam.
+    (* forcing a thunk *)
+    iNext. iSimpl.
+    iApply (wp_bind _ (IFSCtx _ _)).
+    { solve_proper. }
+    iApply (wp_read with "Hctx Hl").
+    iNext. iNext. iIntros "Hl".
+    iApply wp_val. iModIntro.
+    unfold IFSCtx. simpl.
+    rewrite IF_False; last lia.
+    iApply wp_seq.
+    { solve_proper. }
+    iApply (wp_write with "Hctx Hl").
+    iNext. iNext. iIntros "Hl".
+    iApply wp_val. iModIntro.
+    (* doing the glue for the argument *)
+    iApply wp_let.
+    { solve_proper. }
+    iPoseProof (G2 (IT_of_V βv)) as "G2".
+    iSpecialize ("G2" with "[Hb]").
+    { iIntros (ss) "Hss _".
+      iIntros (σ0) "Hs". simpl.
+      iApply wp_val. eauto with iFrame. }
+    iSpecialize ("G2" with "Hctx").
+    iSpecialize ("G2" $! _ emp_ssubst with "Hs []").
+    { iApply ssubst_valid_nil. }
+    iSpecialize ("G2" $! tt with "Hp").
+    iApply (wp_wand with "G2").
+    iIntros (β'v).
+    iDestruct 1 as (_) "[Hb Hp]". iModIntro.
+    simpl. clear σ. iDestruct "Hb" as (σ) "[#Hb Hs]".
+    (* calling the original function *)
+    iApply wp_let.
+    { solve_proper. }
+    iApply (wp_bind _ (AppRSCtx _)).
+    { solve_proper. }
+    iApply (wp_Thunk with "Hctx").
+    { solve_proper. }
+    iNext. iIntros (l') "Hl'".
+    unfold AppRSCtx.
+    iClear "Hl". clear l.
+    iApply fupd_wp.
+    { solve_proper. }
+    iMod (inv_alloc (nroot.@"yolo") _ (∃ n, pointsto l' (Nat n)) with "[Hl']") as "#Hinv".
+    { iNext. iExists _; done. }
+    iPoseProof ("Ha" $! _ (thunkedV (IT_of_V β'v) l') with "Hs [-Has Hp]") as "H1".
+    { iModIntro. iIntros (σ' βn) "Hs Hbm".
+      iDestruct "Hbm" as (m) "Hbm".
+      iIntros (_) "Hp".
+      iApply wp_lam. iNext. iSimpl.
+      iApply (wp_bind _ (IFSCtx _ _)).
+      { solve_proper. }
+      iApply (wp_read_atomic _ _ (⊤∖ nclose (nroot.@"storeE")) with "Hctx").
       { set_solver. }
       iInv (nroot.@"yolo") as (n) "Hl'" "Hcl".
       iModIntro. iExists (Nat n). iFrame.
@@ -998,30 +979,44 @@ Proof.
       iMod ("Hcl" with "[Hl']") as "_".
       { iNext. eauto with iFrame. }
       iModIntro. iApply wp_val.
-      iModIntro. eauto with iFrame.
-    - rewrite IF_True; last lia.
-      iApply wp_err. done. }
-  iModIntro.
-  iApply (wp_wand with "H1").
-  iIntros (γv) "H2".
-  iModIntro. iDestruct "H2" as (σ') "[#H2 Hs]".
-  iPoseProof (G1 (constO (IT_of_V γv))) as "G1".
-  iSpecialize ("G1" with "[H2]").
-  { iIntros (σ0 ss0) "Hs Hp Has". simpl.
-    iApply wp_val. iModIntro. eauto with iFrame. }
-  iSpecialize ("G1" with "Has Hctx Hs").
-  simpl. done.
-Qed.
-
-Arguments interp_tarr {_ _ _ _ _ _ _ _}.
-Arguments interp_ty {_ _ _ _ _ _ _ _} _.
+      iModIntro.
+      unfold IFSCtx. simpl.
+      destruct n as [|n].
+      - rewrite IF_False; last lia.
+        iApply wp_seq.
+        { solve_proper. }
+        iApply (wp_write_atomic _ _ (⊤∖ nclose (nroot.@"storeE")) with "Hctx").
+        { set_solver. }
+        iInv (nroot.@"yolo") as (n) "Hl'" "Hcl".
+        iModIntro. iExists (Nat n). iFrame.
+        iNext. iNext. iIntros "Hl'".
+        iMod ("Hcl" with "[Hl']") as "_".
+        { iNext. eauto with iFrame. }
+        iModIntro. iApply wp_val.
+        iModIntro. iExists tt. eauto with iFrame.
+      - rewrite IF_True; last lia.
+        iApply wp_err. done. }
+    iModIntro.
+    iSpecialize ("H1" $! tt with "Hp").
+    iApply (wp_wand with "H1").
+    iIntros (γv). iDestruct 1 as (_) "[H2 Hp]".
+    iModIntro. simpl. iDestruct "H2" as (σ') "[#H2 Hs]".
+    iPoseProof (G1 (constO (IT_of_V γv))) as "G1".
+    iSpecialize ("G1" with "[H2]").
+    { iIntros (σ0 ss0) "Hs Has". simpl.
+      iApply expr_pred_ret. simpl.
+      eauto with iFrame. }
+    iSpecialize ("G1" with "Hctx Has").
+    iSpecialize ("G1" with "[$Hs $Hp]").
+    simpl. done.
+  Qed.
 
   Lemma glue_to_affine_compatibility {S} (Ω : tyctx S) (τ1 : ty) (τ1' : io_lang.ty)
     (Hconv : ty_conv τ1 τ1') α :
-    io_lang.valid1 rs p empC α τ1' ⊢ valid2 Ω (constO (glue_to_affine Hconv (α ()))) τ1
+    io_valid empC α τ1' ⊢ valid2 Ω (constO (glue_to_affine Hconv (α ()))) τ1
   with glue_from_affine_compatibility (τ1 : ty) (τ1' : io_lang.ty)
     (Hconv : ty_conv τ1 τ1') (α : IT) :
-    valid2 empC (constO α) τ1 ⊢ heap_ctx -∗ io_lang.valid1 rs p empC (constO (glue_from_affine Hconv α)) τ1'.
+    valid2 empC (constO α) τ1 ⊢ heap_ctx -∗ io_valid empC (constO (glue_from_affine Hconv α)) τ1'.
   Proof.
     - destruct Hconv.
       + by iApply compat_glue_to_affine_bool.
@@ -1035,103 +1030,52 @@ Arguments interp_ty {_ _ _ _ _ _ _ _} _.
       + iApply compat_glue_from_affine_bool.
       + iApply compat_glue_from_affine_nat.
       + iApply compat_glue_from_affine_unit.
-      + Opaque io_lang.interp_tarr interp_tarr.
-        iIntros "H #Hctx". iIntros (σ ss) "Hs Hp _".
-        simpl. clear ss.
-        iSpecialize ("H" $! emp_ssubst with "[] Hctx [$Hs $Hp]").
-        { unfold ssubst_valid. simp list_of_tyctx list_of_ssubst.
-          done. }
-        simpl.
-          simpl. iApply wp_let.
-        { solve_proper. }
-        iApply (wp_wand with "H").
-        iIntros (αv) "Ha". iDestruct "Ha" as (σ') "[Ha [Hs Hp]]".
-        iSimpl in "Ha".
-        iSimpl. iModIntro.
-        iApply wp_let.
-        { solve_proper. }
-        iApply (wp_alloc with "Hctx").
-        { solve_proper_please. }
-        iNext. iNext. iIntros (l) "Hl".
-        iApply (wp_val _ _ (thunkedV _ _)). iSimpl.
-        iMod (na_inv_alloc p _ (nroot.@"yolo")
-             (pointsto l (Nat 1) ∨
-             (pointsto l (Nat 0) ∗ interp_tarr (interp_ty τ1) (interp_ty τ2) αv)) with "[Hl Ha]") as "#Hinv".
-        { iNext. iRight. iFrame. }
-        iModIntro. iApply wp_val.
-        iModIntro. iExists _. iFrame.
-        Transparent io_lang.interp_tarr. simpl.
-        iModIntro. clear σ σ'. iIntros (σ βv) "Hs Hp #Hb".
-        iApply wp_lam. iNext.
-        simpl.
-        iApply wp_let.
-        { solve_proper. }
-        iApply wp_lam.
-        iNext. simpl.
-        iApply (wp_bind _ (IFSCtx _ _)).
-        { solve_proper_please. }
-        iApply fupd_wp.
-        { solve_proper. }
-        iMod  (na_inv_acc with "Hinv Hp")
-          as "[Hl [Hp Hcl]]"; [ set_solver | set_solver | ].
-        iModIntro.
-        iDestruct "Hl" as "[Hl | [Hl Ha]]".
-        * iApply (wp_read with "Hctx Hl").
-          iNext. iNext. iIntros "Hl".
-          iApply wp_val.
-          iModIntro.
-          unfold IFSCtx. simpl.
-          rewrite IF_True; last lia.
-          iApply wp_err. done.
-        * iApply (wp_read with "Hctx Hl").
-          iNext. iNext. iIntros "Hl".
-          iApply wp_val.
-          iModIntro.
-          unfold IFSCtx. simpl.
-          rewrite IF_False; last lia.
-          iApply wp_seq.
-          { solve_proper_please. }
-          iApply (wp_write with "Hctx Hl").
-          iNext. iNext. iIntros "Hl".
-          iApply wp_val.
-          iMod ("Hcl" with "[Hl $Hp]") as "Hp".
-          { iNext. iLeft; eauto. }
-          iModIntro.
-          iApply wp_let.
-          { solve_proper. }
-          iSpecialize ("Hb" $! _ (NatV 0) with "Hs Hp []").
-          { eauto with iFrame. }
-          iApply (wp_wand with "Hb").
-          iIntros (γv).
-          iDestruct 1 as (σ') "[Hg [Hst Hp]]".
-          iModIntro. simpl.
-          iApply wp_let.
-          { solve_proper. }
-          iPoseProof (glue_to_affine_compatibility _ empC _ _ Hconv1 (constO (IT_of_V γv))) as "G1".
-          iSpecialize ("G1" with "[Hg]").
-          { iIntros (σ0 ss0) "Hs Hp Has". simpl.
-            iApply wp_val. iModIntro. eauto with iFrame. }
-          iSpecialize ("G1" $! emp_ssubst with "[] Hctx [$Hst $Hp]").
-          { unfold ssubst_valid; simpl. done. }
-          iApply (wp_wand with "G1").
-          clear βv σ'.
-          iIntros (βv). iDestruct 1 as (σ') "[Hb [Hst Hp]]".
-          iModIntro. simpl.
-          iApply wp_let.
-          { solve_proper. }
-          iSpecialize ("Ha" with "Hb [$Hst $Hp]").
-          iApply (wp_wand with "Ha").
-          clear γv σ'.
-          iIntros (γv). iDestruct 1 as (σ') "[Hg [Hst Hp]]".
-          iModIntro.
-          iPoseProof (glue_from_affine_compatibility _ _ Hconv2 (IT_of_V γv)) as "G1".
-          iSpecialize ("G1" with "[Hg] Hctx").
-          { iIntros (ss0) "_ _".
-            iIntros (σ0) "[Hs Hp]". simpl.
-            iApply wp_val. iModIntro. eauto with iFrame. }
-          iSpecialize ("G1" $! _ emp_ssubst with  "Hst Hp []").
-          { unfold io_lang.ssubst_valid; simpl. done. }
-          iApply "G1".
+      + simpl. iApply compat_glue_from_affine_fun.
+        * apply glue_to_affine_compatibility.
+        * apply glue_from_affine_compatibility.
+  Qed.
+
+  Definition interp_typed_expr {S} {Ω : tyctx S} (e : expr S) {τ}
+     (typed : typed_glued Ω e τ) : interp_scope (E:=F) S -n> IT.
+  Proof using rs subReifier0 subReifier1 sz.
+    induction typed.
+    (** glue *)
+    - refine (constO $ glue_to_affine t (io_lang.interp_closed _ e)).
+    (** functions *)
+    - refine (Force ◎ interp_var v).
+    - refine (interp_lam _ IHtyped).
+    - refine (interp_app _ IHtyped1 IHtyped2 ◎ interp_scope_split).
+    (** pairs *)
+    - refine (interp_pair _ IHtyped1 IHtyped2 ◎ interp_scope_split).
+    - refine (interp_destruct _ IHtyped1 IHtyped2 ◎ interp_scope_split).
+    (** references *)
+    - refine (interp_alloc  _ IHtyped).
+    - refine (interp_replace _ IHtyped1 IHtyped2 ◎ interp_scope_split).
+    - refine (interp_dealloc _ IHtyped).
+    (** literals *)
+    - refine (interp_litnat _ n).
+    - refine (interp_litbool _ b).
+    - refine (interp_litunit _).
+  Defined.
+
+  Lemma fundamental_affine_glued {S} (Ω : tyctx S) (e : expr S) τ :
+    ∀ (typed : typed_glued Ω e τ),
+    ⊢ valid2 Ω (interp_typed_expr e typed) τ.
+  Proof.
+    intros typed. induction typed; simpl.
+    - iApply glue_to_affine_compatibility.
+      by iApply fundamental.
+    - by iApply compat_var.
+    - by iApply compat_lam.
+    - by iApply compat_app.
+    - by iApply compat_pair.
+    - by iApply compat_destruct.
+    - by iApply compat_alloc.
+    - by iApply compat_replace.
+    - by iApply compat_dealloc.
+    - by iApply compat_nat.
+    - by iApply compat_bool.
+    - by iApply compat_unit.
   Qed.
 
 End glue.
